update all case of Typing.env_insert_preservation

dsn/Lang/String/Basic.lean
@@ -8,7 +8,6 @@ import Lang.List.Basic
 
 set_option pp.fieldNotation false
 
-
 namespace Lang
 
 #check Lean.mkFreshId
@@ -113,18 +112,21 @@ theorem String.length_repr_non_zero :
 
 
 theorem String.foldl_append_seed_exclusion :
-List.foldl (fun r s => r ++ s) (pre ++ name ++ post) names ++ Nat.repr i ≠ name
+name_prefix ++ List.foldl (fun r s => r ++ s) (pre ++ name ++ post) names ++ Nat.repr i ≠ name
 := by cases names with
 | nil =>
   intro h0
   apply congrArg String.length at h0
   simp at h0
-  have h2 :
+  have it :
     String.length pre + String.length name =
     String.length name + String.length pre
   := by exact Nat.add_comm (String.length pre) (String.length name)
-  rw [h2] at h0 ; clear h2
-  simp [Nat.add_assoc] at h0
+  simp [it] at h0 ; clear it
+  rw [Nat.add_left_comm] at h0
+  rw [Nat.add_assoc] at h0
+  rw [Nat.add_assoc] at h0
+  simp at h0
   have ⟨h3,h4,h5⟩ := h0
   clear h0 h3
   apply String.length_repr_non_zero h5
@@ -138,7 +140,7 @@ List.foldl (fun r s => r ++ s) (pre ++ name ++ post) names ++ Nat.repr i ≠ nam
   apply String.foldl_append_seed_exclusion
 
 theorem String.foldl_append_list_exclusion :
-List.foldl (fun r s => r ++ s) name names ++ Nat.repr i ∉ names
+name_prefix ++ List.foldl (fun r s => r ++ s) name names ++ Nat.repr i ∉ names
 := by cases names with
 | nil =>
   simp
@@ -185,21 +187,54 @@ List.foldl (fun r s => r ++ s) name names ++ Nat.repr i ∉ names
 --     }
 --   }
 
-theorem String.fresh_names n names':
+
+def String.recursive_prefix := "_r_"
+
+def String.namespace_recursive (name : String) : Prop :=
+  String.IsPrefix recursive_prefix name
+
+
+def String.no_namespace_recursive (names : List String) : Prop :=
+  ∀ name ∈ names, ¬ String.namespace_recursive name
+
+
+def String.quantified_prefix := "_q_"
+def String.namespace_quantified (name : String) : Prop :=
+  String.IsPrefix quantified_prefix name
+
+
+example :
+  ∀ name,
+    String.IsPrefix String.quantified_prefix name →
+    ¬ String.IsPrefix String.recursive_prefix name
+:= by
+  simp [String.quantified_prefix, String.recursive_prefix, String.IsPrefix]
+  intro name h0 h1
+
+  simp [List.IsPrefix] at h0 h1
+  have ⟨xs,h2⟩ := h0
+  have ⟨ys,h3⟩ := h1
+  simp [←h2] at h3
+
+
+theorem String.fresh_names n names' name_prefix :
   ∃ names : List String,
   List.length names = n ∧
-  List.Disjoint names names'
+  List.Disjoint names names' ∧
+  (∀ name ∈ names, String.IsPrefix name_prefix name)
   /- NOTE: uniqueness of names isn't necessary
   -- ∧ List.Pairwise (fun x y => x ≠ y) names
   -/
 := by
-  exists (List.map (fun i => (String.join names') ++ (Nat.repr i)) (List.range n))
+  exists (List.map (fun i => name_prefix ++ (String.join names') ++ (Nat.repr i)) (List.range n))
 
   apply And.intro
   { simp }
+  apply And.intro
   { simp [List.Disjoint, String.join]
-    intro i h0
-    exact foldl_append_list_exclusion
+    intro i h0 h1
+    apply String.foldl_append_list_exclusion h1
   }
+  { simp [String.IsPrefix] }
 
 end Lang
