dsn/Lang/Typing/Basic.lean
@@ -41,74 +41,74 @@ theorem Stable.subject_expansion :
 
 
 mutual
-  /- NOTE: tvars holds temporary vars that may be used for applying rules to instances -/
-  def Subtyping (tvars : List String) (am : List (String × (Expr → Prop))) (left : Typ) (right : Typ) : Prop :=
-    ∀ e, Typing tvars am e left → Typing tvars am e right
+  def Subtyping (am : List (String × (Expr → Prop))) (left : Typ) (right : Typ) : Prop :=
+    ∀ e, Typing am e left → Typing am e right
   termination_by (Typ.size left + Typ.size right, 0)
   decreasing_by
     all_goals (apply Prod.Lex.left ; simp [Typ.zero_lt_size])
 
 
-  def MultiSubtyping (tvars : List String) (am : List (String × (Expr → Prop))) : List (Typ × Typ) → Prop
+  def MultiSubtyping (am : List (String × (Expr → Prop))) : List (Typ × Typ) → Prop
   | .nil => True
   | .cons (left, right) remainder =>
-    Subtyping tvars am left right ∧ MultiSubtyping tvars am remainder
+    Subtyping am left right ∧ MultiSubtyping am remainder
   termination_by sts => (List.pair_typ_size sts, 0)
   decreasing_by
     all_goals (apply Prod.Lex.left ; simp [List.pair_typ_size, List.pair_typ_zero_lt_size, Typ.zero_lt_size])
 
-  def PosMonotonic (name : String) (tvars : List String) (am : List (String × (Expr → Prop))) (t : Typ) : Prop :=
+  def PosMonotonic (name : String) (am : List (String × (Expr → Prop))) (t : Typ) : Prop :=
     (∀ P0 P1 : Expr → Prop,
       Stable P0 → Stable P1 →
       (∀ e, P0 e → P1 e) →
-      (∀ e , Typing tvars ((name,P0)::am) e t → Typing tvars ((name,P1)::am) e t)
+      (∀ e , Typing ((name,P0)::am) e t → Typing ((name,P1)::am) e t)
     )
   termination_by (Typ.size t, 1)
 
 
-  def Typing (tvars : List String) (am : List (String × (Expr → Prop))) (e : Expr) : Typ → Prop
+  -- TODO: need to switch back to using recursive namespace;
+  def Typing (am : List (String × (Expr → Prop))) (e : Expr) : Typ → Prop
   | .var id => Safe e ∧ ∃ P, Stable P ∧ Prod.find id am = some P ∧ P e
   | .bvar _ => False
   | .bot => False
   | .top => Safe e
-  | .iso l t => Safe e ∧ Typing tvars am (.extract e l) t
-  | .entry l t => Safe e ∧ Typing tvars am (.project e l) t
+  | .iso l t => Safe e ∧ Typing am (.extract e l) t
+  | .entry l t => Safe e ∧ Typing am (.project e l) t
   | .path left right =>
     Safe e ∧
-    ∀ arg , Typing tvars am arg left → Typing tvars am (.app e arg) right
-  | .unio left right => Typing tvars am e left ∨ Typing tvars am e right
-  | .inter left right => Typing tvars am e left ∧ Typing tvars am e right
-  | .diff left right => Typing tvars am e left ∧ ¬ (Typing tvars am e right)
+    ∀ arg , Typing am arg left → Typing am (.app e arg) right
+  | .unio left right => Typing am e left ∨ Typing am e right
+  | .inter left right => Typing am e left ∧ Typing am e right
+  | .diff left right => Typing am e left ∧ ¬ (Typing am e right)
 
   | .exi bs cs body =>
     (∀ a ∈ bs , a = "") ∧
     ∀ names,
     List.length names = List.length bs →
-    List.Disjoint names tvars →
+    String.no_namespace_recursive names →
     List.Disjoint names (Prod.dom am) →
       ∃ am' , Prod.dom am' = names ∧
-      (MultiSubtyping tvars (am' ++ am) (Typ.constraints_instantiate 0 (List.map Typ.var names) cs)) ∧
-      (Typing tvars (am' ++ am) e (Typ.instantiate 0 (List.map Typ.var names) body))
+      (MultiSubtyping (am' ++ am) (Typ.constraints_instantiate 0 (List.map Typ.var names) cs)) ∧
+      (Typing (am' ++ am) e (Typ.instantiate 0 (List.map Typ.var names) body))
 
   | .all bs cs body =>
     Safe e ∧
     (∀ a ∈ bs , a = "") ∧
     ∃ names,
     List.length names = List.length bs ∧
-    List.Disjoint names tvars ∧
+    String.no_namespace_recursive names ∧
     List.Disjoint names (Prod.dom am) ∧
     ∀ am' , Prod.dom am' = names →
-    (MultiSubtyping tvars (am' ++ am) (Typ.constraints_instantiate 0 (List.map Typ.var names) cs)) →
-      (Typing tvars (am' ++ am) e (Typ.instantiate 0 (List.map Typ.var names) body))
+    (MultiSubtyping (am' ++ am) (Typ.constraints_instantiate 0 (List.map Typ.var names) cs)) →
+      (Typing (am' ++ am) e (Typ.instantiate 0 (List.map Typ.var names) body))
   | .lfp a body =>
     Safe e ∧
     a = "" ∧
-    ∀ name , name ∉ tvars → name ∉ (Prod.dom am) →
-      PosMonotonic name tvars am (Typ.instantiate 0 [.var name] body) ∧
+    ∀ name , String.namespace_recursive name → name ∉ (Prod.dom am ∩ Typ.free_vars body) →
+      PosMonotonic name am (Typ.instantiate 0 [.var name] body) ∧
       /- infimum of -/
       (∀ P, Stable P →
         /- pre-fixed point -/
-        (∀ e', Typing tvars ((name,P) :: am) e' (Typ.instantiate 0 [.var name] body) → P e') →
+        (∀ e', Typing ((name,P) :: am) e' (Typ.instantiate 0 [.var name] body) → P e') →
         P e
       )
   termination_by t => (Typ.size t, 0)
@@ -124,31 +124,31 @@ mutual
 end
 
 
-def NegMonotonic (name : String) (tvars : List String) (am : List (String × (Expr → Prop))) (t : Typ) : Prop :=
+def NegMonotonic (name : String) (am : List (String × (Expr → Prop))) (t : Typ) : Prop :=
   (∀ P0 P1 : Expr → Prop,
     Stable P0 → Stable P1 →
     (∀ e, P0 e → P1 e) →
-    (∀ e , Typing tvars ((name,P1)::am) e t → Typing tvars ((name,P0)::am) e t)
+    (∀ e , Typing ((name,P1)::am) e t → Typing ((name,P0)::am) e t)
   )
 
-def Monotonic (polarity : Bool) (name : String) (tvars : List String) (am : List (String × (Expr → Prop))) (t : Typ) : Prop :=
-  (polarity = true ∧ PosMonotonic name tvars am t) ∨
-  (polarity = false ∧ NegMonotonic name tvars am t)
+def Monotonic (polarity : Bool) (name : String) (am : List (String × (Expr → Prop))) (t : Typ) : Prop :=
+  (polarity = true ∧ PosMonotonic name am t) ∨
+  (polarity = false ∧ NegMonotonic name am t)
 
-def MultiMonotonic (polarity : Bool) (name : String) (tvars : List String) (am : List (String × (Expr → Prop))) (cs : List (Typ × Typ)) : Prop :=
-  ∀ lower upper, (lower,upper) ∈ cs → Monotonic (not polarity) name tvars am lower ∧ Monotonic polarity name tvars am upper
+def MultiMonotonic (polarity : Bool) (name : String) (am : List (String × (Expr → Prop))) (cs : List (Typ × Typ)) : Prop :=
+  ∀ lower upper, (lower,upper) ∈ cs → Monotonic (not polarity) name am lower ∧ Monotonic polarity name am upper
 
-def EitherMultiMonotonic (name : String) (tvars : List String) (am : List (String × (Expr → Prop))) (cs : List (Typ × Typ)) : Prop :=
-  MultiMonotonic .true name tvars am cs ∨ MultiMonotonic .false name tvars am cs
+def EitherMultiMonotonic (name : String) (am : List (String × (Expr → Prop))) (cs : List (Typ × Typ)) : Prop :=
+  MultiMonotonic .true name am cs ∨ MultiMonotonic .false name am cs
 
 
 def MultiTyping
-  (tvars : List String) (tam : List (String × (Expr → Prop))) (eam : List (String × Expr)) (context : List (String × Typ)) : Prop
-:= ∀ {x t}, Prod.find x context = .some t → ∃ e, (Prod.find x eam) = .some e ∧ Typing tvars tam e t
+  (tam : List (String × (Expr → Prop))) (eam : List (String × Expr)) (context : List (String × Typ)) : Prop
+:= ∀ {x t}, Prod.find x context = .some t → ∃ e, (Prod.find x eam) = .some e ∧ Typing tam e t
 
 
 theorem Typing.safety :
-  Typing tvars am e t → Safe e
+  Typing am e t → Safe e
 := by cases t with
 | bvar i =>
   simp [Typing]
@@ -190,14 +190,24 @@ theorem Typing.safety :
   apply Typing.safety h0
 | all bs cs body =>
   simp [Typing]
-  intro h0 h1 names h2 h3 tvars_disjoint h4
+  intro h0 h1 names h2 h3 h4 h5
   exact h0
 | exi bs cs body =>
   simp [Typing]
   intro h0 h1 e' h2
-  have ⟨names,h3,h4⟩ := String.fresh_names (List.length bs) (tvars ++ Prod.dom am)
-  have ⟨h4A,h4B⟩ := Iff.mp List.disjoint_append_right h4
-  have ⟨am',h5,h6,h7⟩ := h1 names h3 h4A h4B
+  have ⟨names,h3,h4A, h4B⟩ := String.fresh_names (List.length bs) (Prod.dom am) String.quantified_prefix
+
+  have h4 : String.no_namespace_recursive names := by
+    simp [String.no_namespace_recursive, String.namespace_recursive, String.recursive_prefix]
+    simp [String.IsPrefix, List.IsPrefix]
+    intro name h5 xs
+    specialize h4B name h5
+    simp [String.quantified_prefix, String.IsPrefix, List.IsPrefix] at h4B
+    have ⟨ys,h6⟩ := h4B
+    rw [←h6]
+    simp
+
+  have ⟨am',h5,h6,h7⟩ := h1 names h3 h4 h4A
   apply Typing.safety h7 _ h2
 | lfp x body =>
   simp [Typing]
@@ -218,7 +228,7 @@ decreasing_by
 
 
 theorem Typing.progress :
-  Typing tvars am e t → Expr.valued e ∨ ∃ e', NStep e e'
+  Typing am e t → Expr.valued e ∨ ∃ e', NStep e e'
 := by
   intro h0
   apply Safe.progress
@@ -228,7 +238,7 @@ theorem Typing.progress :
 mutual
   theorem Typing.subject_reduction
     (transition : NStep e e')
-  : Typing tvars am e t → Typing tvars am e' t
+  : Typing am e t → Typing am e' t
   := by cases t with
   | bvar i =>
     simp [Typing]
@@ -360,7 +370,7 @@ mutual
 
   theorem Typing.subject_expansion
     (transition : NStep e e')
-  : Typing tvars am e' t → Typing tvars am e t
+  : Typing am e' t → Typing am e t
   := by cases t with
   | bvar i =>
     simp [Typing]
@@ -505,7 +515,7 @@ end
 
 theorem Typing.refl_trans_left_subject_expansion
   (transition : ReflTransLeft NStep e e')
-: Typing tvars am e' t → Typing tvars am e t
+: Typing am e' t → Typing am e t
 := by induction transition with
 | refl =>
   intro h0 ; exact h0
@@ -516,14 +526,14 @@ theorem Typing.refl_trans_left_subject_expansion
 
 theorem Typing.refl_trans_subject_expansion
   (transition : ReflTrans NStep e e')
-: Typing tvars am e' t → Typing tvars am e t
+: Typing am e' t → Typing am e t
 := by
   apply Typing.refl_trans_left_subject_expansion
   exact ReflTrans.reverse transition
 
 theorem Typing.refl_trans_subject_reduction
   (transition : ReflTrans NStep e e')
-: Typing tvars am e t → Typing tvars am e' t
+: Typing am e t → Typing am e' t
 := by induction transition with
 | refl =>
   intro h0 ; exact h0
@@ -532,39 +542,43 @@ theorem Typing.refl_trans_subject_reduction
   apply ih ; clear ih
   apply Typing.subject_reduction h0 h2
 
-/-
--- TODO:
---
-
-  theorem Typing.env_insert_reflection :
-    name ∉ Typ.free_vars t →
-    name ∈ tvars →
-    Typing tvars (m0 ++ (name,P) :: m1) e t →
-    Typing tvars (m0 ++ m1) e t
-  := by sorry
-
-  theorem Typing.env_insert_preservation :
-    name ∉ Typ.free_vars t →
-    name ∈ tvars →
-    Typing tvars (m0 ++ m1) e t
-    Typing tvars (m0 ++ (name,P) :: m1) e t →
-  := by sorry
-
--/
-
 mutual
+
+  theorem MultiSubtyping.env_insert_reflection :
+    name ∉ Typ.list_prod_free_vars cs →
+    String.namespace_recursive name →
+    MultiSubtyping (m0 ++ (name,P) :: m1) cs →
+    MultiSubtyping (m0 ++ m1) cs
+  := by sorry
+  termination_by sts => (List.pair_typ_size cs, 0)
+  decreasing_by
+    all_goals sorry
+
+  theorem MultiSubtyping.env_insert_preservation :
+    name ∉ Typ.list_prod_free_vars cs →
+    String.namespace_recursive name →
+    MultiSubtyping (m0 ++ m1) cs →
+    ∀ P, MultiSubtyping (m0 ++ (name,P) :: m1) cs
+  := by sorry
+  termination_by sts => (List.pair_typ_size cs, 0)
+  decreasing_by
+    all_goals sorry
+
   theorem Typing.env_insert_reflection :
     name ∉ Typ.free_vars t →
-    name ∈ tvars →
-    Typing tvars (m0 ++ (name,P) :: m1) e t →
-    Typing tvars (m0 ++ m1) e t
+    String.namespace_recursive name →
+    Typing (m0 ++ (name,P) :: m1) e t →
+    Typing (m0 ++ m1) e t
   := by sorry
+  termination_by (Typ.size t, 0)
+  decreasing_by
+    all_goals sorry
 
   theorem Typing.env_insert_preservation :
     name ∉ Typ.free_vars t →
-    name ∈ tvars →
-    Typing tvars (m0 ++ m1) e t →
-    ∀ P, Typing tvars (m0 ++ (name,P) :: m1) e t
+    String.namespace_recursive name →
+    Typing (m0 ++ m1) e t →
+    ∀ P, Typing (m0 ++ (name,P) :: m1) e t
   := by cases t with
   | bvar i =>
     simp [Typing]
@@ -585,6 +599,10 @@ mutual
       simp [h0]
       exact h4
     }
+  | bot =>
+    simp [Typing]
+  | top =>
+    simp [Typing]
   | iso l body =>
     simp [Typing, Typ.free_vars]
     intro h0 h1 h2 h3 P
@@ -595,62 +613,120 @@ mutual
     intro h0 h1 h2 h3 P
     simp [*]
     apply Typing.env_insert_preservation h0 h1 h3
-  -- | all bs cs body =>
-  --   simp [Typing, Typ.free_vars]
-  --   intro h0 h1 h2 h3 h4 names h5 h6 h7 h8 P
-  --   simp [*]
-  --   apply And.intro h4
-  --   exists names
-  --   simp [*]
-  --   apply And.intro
-  --   {
-  --     simp [List.Disjoint]
-  --     intro name' h9
-  --     simp [Prod.dom]
-  --     apply And.intro
-  --     {
-  --       simp [List.Disjoint, Prod.dom] at h7
-  --       intro P' h10
-  --       have ⟨h11,h12⟩ := h7 h9
-  --       exact h11 P' h10
-  --     }
-  --     apply And.intro
-  --     {
-  --       intro h10
-  --       simp [List.Disjoint] at h6
-  --       apply h6 h9
-  --       rw [h10]
-  --       exact h2
-  --     }
-  --     {
-  --       simp [List.Disjoint, Prod.dom] at h7
-  --       intro P' h10
-  --       have ⟨h11,h12⟩ := h7 h9
-  --       exact h12 P' h10
-  --     }
-  --   }
-  --   sorry
+  | path antec conseq =>
+    simp [Typing, Typ.free_vars]
+    intro h0 h1 h2 h3 h4 P
+    simp [*]
+    intro arg h7
+    apply Typing.env_insert_preservation h1 h2
+    apply h4
+    apply Typing.env_insert_reflection h0 h2 h7
+  | unio left right =>
+    simp [Typing, Typ.free_vars]
+    intro h0 h1 h2 h3 P
+    cases h3 with
+    | inl h4 =>
+      apply Or.inl
+      apply Typing.env_insert_preservation h0 h2 h4
+    | inr h4 =>
+      apply Or.inr
+      apply Typing.env_insert_preservation h1 h2 h4
+  | inter left right =>
+    simp [Typing, Typ.free_vars]
+    intro h0 h1 h2 h3 h4 P
+    apply And.intro
+    { apply Typing.env_insert_preservation h0 h2 h3 }
+    { apply Typing.env_insert_preservation h1 h2 h4 }
+  | diff minu subtra =>
+    simp [Typing, Typ.free_vars]
+    intro h0 h1 h2 h3 h4 P
+    apply And.intro
+    { apply Typing.env_insert_preservation h0 h2 h3 }
+    { intro h5
+      apply h4
+      apply Typing.env_insert_reflection h1 h2 h5
+    }
+
+  | all bs cs body =>
+    simp [Typing, Typ.free_vars]
+    intro h0 h1 h2 h3 h4 names h5 h6 h7 h8 P
+    simp [*]
+    apply And.intro h4
+    exists names
+    simp [*]
+    apply And.intro
+    {
+      simp [List.Disjoint]
+      intro name' h9
+      simp [Prod.dom]
+      apply And.intro
+      {
+        simp [List.Disjoint, Prod.dom] at h7
+        intro P' h10
+        have ⟨h11,h12⟩ := h7 h9
+        exact h11 P' h10
+      }
+      apply And.intro
+      {
+        intro h10
+        simp [String.no_namespace_recursive] at h6
+        apply h6 name
+        { rw [←h10] ; exact h9 }
+        { exact h2 }
+      }
+      {
+        simp [List.Disjoint, Prod.dom] at h7
+        intro P' h10
+        have ⟨h11,h12⟩ := h7 h9
+        exact h12 P' h10
+      }
+    }
+    {
+      intro m h9 h10
+      rw [←List.append_assoc]
+      apply Typing.env_insert_preservation
+      { intro h11
+        apply Typ.free_vars_instantiate_upper_bound at h11
+        simp at h11
+        cases h11 with
+        | inl h12 =>
+          exact h1 h12
+        | inr h12 =>
+          simp [Typ.free_vars] at h12
+          simp [String.no_namespace_recursive] at h6
+          apply h6 name h12
+          apply h2
+      }
+      { exact h2 }
+      {
+        rw [List.append_assoc]
+        apply h8 _ h9
+        rw [←List.append_assoc]
+        apply MultiSubtyping.env_insert_reflection
+        { intro h11
+          apply Typ.list_prod_free_vars_instantiate_upper_bound at h11
+          simp at h11
+          cases h11 with
+          | inl h12 =>
+            exact h0 h12
+          | inr h12 =>
+            simp [Typ.free_vars] at h12
+            simp [String.no_namespace_recursive] at h6
+            apply h6 name h12
+            apply h2
+        }
+        { exact h2 }
+        { rw [List.append_assoc]
+          exact h10
+        }
+      }
+    }
   | _ => sorry
+  termination_by (Typ.size t, 0)
+  decreasing_by
+    all_goals sorry
 end
 
-
--- The following is not provable
--- mutual
---   theorem Typing.env_append_suffix_reflection :
---     List.Disjoint (Prod.dom m0) (Typ.free_vars t) →
---     -- (∀ name ∈ Prod.dom m0, name ∈ tvars ∨ ) →
---     Typing tvars (m0 ++ m1) e t →
---     Typing tvars m1 e t
---   := by
---     sorry
-
---   theorem Typing.env_append_suffix_preservation :
---     List.Disjoint (Prod.dom m0) (Typ.free_vars t) →
---     Typing tvars m1 e t →
---     Typing tvars (m0 ++ m1) e t
---   := by
---     sorry
--- end
 
 
 -- theorem Typing.env_cons_swap :
